p256: use addition chain for finv

code/ecdsap256/Hacl.Impl.P256.Finv.fst
@@ -70,22 +70,170 @@ let mk_p256_prime_concrete_ops : BE.concrete_ops U64 4ul 0ul = {
 }
 
 
+val fsquare_times_in_place (out:felem) (b:size_t) : Stack unit
+  (requires fun h ->
+    live h out /\ as_nat h out < S.prime)
+  (ensures  fun h0 _ h1 -> modifies (loc out) h0 h1 /\
+    as_nat h1 out < S.prime /\
+    fmont_as_nat h1 out == SI.fsquare_times (fmont_as_nat h0 out) (v b))
+
+[@CInline]
+let fsquare_times_in_place out b =
+  let h0 = ST.get () in
+  SE.exp_pow2_lemma SI.mk_nat_mod_concrete_ops (fmont_as_nat h0 out) (v b);
+  BE.lexp_pow2_in_place 4ul 0ul mk_p256_prime_concrete_ops (null uint64) out b
+
+
 val fsquare_times (out a:felem) (b:size_t) : Stack unit
   (requires fun h ->
     live h out /\ live h a /\ disjoint out a /\
     as_nat h a < S.prime)
   (ensures  fun h0 _ h1 -> modifies (loc out) h0 h1 /\
+    as_nat h1 out < S.prime /\
     fmont_as_nat h1 out == SI.fsquare_times (fmont_as_nat h0 a) (v b))
 
 [@CInline]
 let fsquare_times out a b =
   let h0 = ST.get () in
-  BE.lexp_pow2 4ul 0ul mk_p256_prime_concrete_ops (null uint64) a b out;
+  SE.exp_pow2_lemma SI.mk_nat_mod_concrete_ops (fmont_as_nat h0 a) (v b);
+  BE.lexp_pow2 4ul 0ul mk_p256_prime_concrete_ops (null uint64) a b out
+
+
+inline_for_extraction noextract
+val finv_30 (x30 x2 tmp1 tmp2 a:felem) : Stack unit
+  (requires fun h ->
+    live h a /\ live h x30 /\ live h x2 /\ live h tmp1 /\ live h tmp2 /\
+    disjoint a x30 /\ disjoint a x2 /\ disjoint a tmp1 /\ disjoint a tmp2 /\
+    disjoint x30 x2 /\ disjoint x30 tmp1 /\ disjoint x30 tmp2 /\
+    disjoint x2 tmp1 /\ disjoint x2 tmp2 /\ disjoint tmp1 tmp2 /\
+    as_nat h a < S.prime)
+  (ensures fun h0 _ h1 -> modifies (loc x30 |+| loc x2 |+| loc tmp1 |+| loc tmp2) h0 h1 /\
+    as_nat h1 x30 < S.prime /\ as_nat h1 x2 < S.prime /\
+    (let f = fmont_as_nat h0 a in
+    let x2_s = S.fmul (SI.fsquare_times f 1) f in
+    let x3_s = S.fmul (SI.fsquare_times x2_s 1) f in
+    let x6_s = S.fmul (SI.fsquare_times x3_s 3) x3_s in
+    let x12_s = S.fmul (SI.fsquare_times x6_s 6) x6_s in
+    let x15_s = S.fmul (SI.fsquare_times x12_s 3) x3_s in
+    let x30_s = S.fmul (SI.fsquare_times x15_s 15) x15_s in
+    fmont_as_nat h1 x30 = x30_s /\ fmont_as_nat h1 x2 = x2_s))
+
+let finv_30 x30 x2 tmp1 tmp2 a =
+  let h0 = ST.get () in
+  fsquare_times x2 a 1ul;
+  fmul x2 x2 a;
   let h1 = ST.get () in
-  assert (fmont_as_nat h1 out == LE.exp_pow2 SI.nat_mod_comm_monoid (fmont_as_nat h0 a) (v b));
-  SE.exp_pow2_lemma SI.mk_nat_mod_concrete_ops (fmont_as_nat h0 a) (v b)
+  assert (fmont_as_nat h1 x2 ==
+    S.fmul (SI.fsquare_times (fmont_as_nat h0 a) 1) (fmont_as_nat h0 a));
+
+  fsquare_times x30 x2 1ul;
+  fmul x30 x30 a;
+  let h2 = ST.get () in
+  assert (fmont_as_nat h2 x30 == // x3
+    S.fmul (SI.fsquare_times (fmont_as_nat h1 x2) 1) (fmont_as_nat h0 a));
+
+  fsquare_times tmp1 x30 3ul;
+  fmul tmp1 tmp1 x30;
+  let h3 = ST.get () in
+  assert (fmont_as_nat h3 tmp1 == // x6
+    S.fmul (SI.fsquare_times (fmont_as_nat h2 x30) 3) (fmont_as_nat h2 x30));
+
+  fsquare_times tmp2 tmp1 6ul;
+  fmul tmp2 tmp2 tmp1;
+  let h4 = ST.get () in
+  assert (fmont_as_nat h4 tmp2 == // x12
+    S.fmul (SI.fsquare_times (fmont_as_nat h3 tmp1) 6) (fmont_as_nat h3 tmp1));
+
+  fsquare_times tmp1 tmp2 3ul;
+  fmul tmp1 tmp1 x30;
+  let h5 = ST.get () in
+  assert (fmont_as_nat h5 tmp1 == // x15
+    S.fmul (SI.fsquare_times (fmont_as_nat h4 tmp2) 3) (fmont_as_nat h2 x30));
+
+  fsquare_times x30 tmp1 15ul;
+  fmul x30 x30 tmp1;
+  let h6 = ST.get () in
+  assert (fmont_as_nat h6 x30 == // x30
+    S.fmul (SI.fsquare_times (fmont_as_nat h5 tmp1) 15) (fmont_as_nat h5 tmp1))
 
 
+inline_for_extraction noextract
+val finv_256 (x256 x2 x30 a:felem) : Stack unit
+  (requires fun h ->
+    live h a /\ live h x30 /\ live h x2 /\ live h x256 /\
+    disjoint a x30 /\ disjoint a x2 /\ disjoint a x256 /\
+    disjoint x30 x2 /\ disjoint x30 x256 /\ disjoint x2 x256 /\
+    as_nat h a < S.prime /\ as_nat h x30 < S.prime /\ as_nat h x2 < S.prime)
+  (ensures fun h0 _ h1 -> modifies (loc x256 |+| loc x2) h0 h1 /\
+    as_nat h1 x256 < S.prime /\
+   (let f = fmont_as_nat h0 a in
+    let x30 = fmont_as_nat h0 x30 in
+    let x2 = fmont_as_nat h0 x2 in
+    let x32_s = S.fmul (SI.fsquare_times x30 2) x2 in
+    let x64_s = S.fmul (SI.fsquare_times x32_s 32) f in
+    let x192_s = S.fmul (SI.fsquare_times x64_s 128) x32_s in
+    let x224_s = S.fmul (SI.fsquare_times x192_s 32) x32_s in
+    let x254_s = S.fmul (SI.fsquare_times x224_s 30) x30 in
+    let x256_s = S.fmul (SI.fsquare_times x254_s 2) f in
+    fmont_as_nat h1 x256 = x256_s))
+
+let finv_256 x256 x2 x30 a =
+  let h0 = ST.get () in
+  fsquare_times x256 x30 2ul;
+  fmul x256 x256 x2;
+  let h1 = ST.get () in
+  assert (fmont_as_nat h1 x256 == // x32
+    S.fmul (SI.fsquare_times (fmont_as_nat h0 x30) 2) (fmont_as_nat h0 x2));
+
+  fsquare_times x2 x256 32ul;
+  fmul x2 x2 a;
+  let h2 = ST.get () in
+  assert (fmont_as_nat h2 x2 == // x64
+    S.fmul (SI.fsquare_times (fmont_as_nat h1 x256) 32) (fmont_as_nat h0 a));
+
+  fsquare_times_in_place x2 128ul;
+  fmul x2 x2 x256;
+  let h3 = ST.get () in
+  assert (fmont_as_nat h3 x2 == // x192
+    S.fmul (SI.fsquare_times (fmont_as_nat h2 x2) 128) (fmont_as_nat h1 x256));
+
+  fsquare_times_in_place x2 32ul;
+  fmul x2 x2 x256;
+  let h4 = ST.get () in
+  assert (fmont_as_nat h4 x2 == // x224
+    S.fmul (SI.fsquare_times (fmont_as_nat h3 x2) 32) (fmont_as_nat h1 x256));
+
+  fsquare_times_in_place x2 30ul;
+  fmul x2 x2 x30;
+  let h5 = ST.get () in
+  assert (fmont_as_nat h5 x2 == // x254
+    S.fmul (SI.fsquare_times (fmont_as_nat h4 x2) 30) (fmont_as_nat h0 x30));
+
+  fsquare_times_in_place x2 2ul;
+  fmul x256 x2 a;
+  let h6 = ST.get () in
+  assert (fmont_as_nat h6 x256 == // x256
+    S.fmul (SI.fsquare_times (fmont_as_nat h5 x2) 2) (fmont_as_nat h0 a))
+
+
+[@CInline]
+let finv res a =
+  let h0 = ST.get () in
+  push_frame ();
+  let tmp  = create 16ul (u64 0) in
+  let x30  = sub tmp 0ul 4ul in
+  let x2   = sub tmp 4ul 4ul in
+  let tmp1 = sub tmp 8ul 4ul in
+  let tmp2 = sub tmp 12ul 4ul in
+  finv_30 x30 x2 tmp1 tmp2 a;
+  finv_256 tmp1 x2 x30 a;
+  copy res tmp1;
+  let h1 = ST.get () in
+  assert (fmont_as_nat h1 res == SI.finv (fmont_as_nat h0 a));
+  SI.finv_is_finv_lemma (fmont_as_nat h0 a);
+  pop_frame ()
+
+//--------------------------------
 // TODO: rm
 val fexp_vartime (out a b:felem) : Stack unit
   (requires fun h ->
@@ -113,36 +261,7 @@ let fexp_vartime out a b =
   M.lemma_pow_mod #S.prime (fmont_as_nat h0 a) (as_nat h0 b)
 
 
-//--------------------------------
 // TODO: use an addition chain from Hacl.Spec.P256.Finv
-inline_for_extraction noextract
-val make_prime_minus_2: b:felem -> Stack unit
-  (requires fun h -> live h b)
-  (ensures  fun h0 _ h1 -> modifies (loc b) h0 h1 /\
-    as_nat h1 b == S.prime - 2)
-
-let make_prime_minus_2 b =
-  // 0xffffffff00000001000000000000000000000000fffffffffffffffffffffffd
-  [@inline_let] let b0 = u64 0xfffffffffffffffd in
-  [@inline_let] let b1 = u64 0xffffffff in
-  [@inline_let] let b2 = u64 0x0 in
-  [@inline_let] let b3 = u64 0xffffffff00000001 in
-  assert_norm (v b0 + v b1 * pow2 64 + v b2 * pow2 128 + v b3 * pow2 192 = S.prime - 2);
-  bn_make_u64_4 b b0 b1 b2 b3
-
-
-[@CInline]
-let finv res a =
-  push_frame ();
-  let b = create 4ul (u64 0) in
-  make_prime_minus_2 b;
-
-  let tmp = create 4ul (u64 0) in
-  copy tmp a;
-  fexp_vartime res tmp b;
-  pop_frame ()
-
-
 inline_for_extraction noextract
 val make_prime_plus_1_div_4: b:felem -> Stack unit
   (requires fun h -> live h b)
